WIP

theories/sim/local_adequacy.v
@@ -2,6 +2,99 @@ From Coq Require Import Program.Equality Lia.
 From Paco Require Import paco.
 
 From stbor.lang Require Import steps_wf.
-From stbor.sim Require Import global invariant sflib.
+From stbor.sim Require Import behavior global local invariant sflib global_adequacy.
 
 Set Default Proof Using "Type".
+
+Section local.
+Context {A: ucmraT}.
+Variable (wsat: A → state → state → Prop).
+Variable (vrel: A → expr → expr → Prop).
+Variable (fns fnt: fn_env).
+
+Record frame: Type := mk_frame {
+  rc: A;
+  K_src: list (ectxi_language.ectx_item (bor_ectxi_lang fns));
+  K_tgt: list (ectxi_language.ectx_item (bor_ectxi_lang fnt));
+}.
+
+Inductive sim_local_frames:
+  forall (r_f:A)
+    (K_src: list (ectxi_language.ectx_item (bor_ectxi_lang fns)))
+    (K_tgt: list (ectxi_language.ectx_item (bor_ectxi_lang fnt)))
+    (frames:list frame),
+    Prop :=
+| sim_local_frames_nil
+    r_f
+  : sim_local_frames r_f nil nil nil
+| sim_local_frames_cons
+    r_f K_f_src K_f_tgt
+    frame frames
+    (FRAMES: sim_local_frames r_f K_f_src K_f_tgt frames)
+    (CONTINUATION:
+       ∀ r_f' r' v_src v_tgt σ_src' σ_tgt'
+         (* For any new resource r' and frame r_f' that are compatible with
+             our local resource r and have world satisfaction *)
+         (VALID': ✓ (r_f' ⋅ (frame.(rc) ⋅ r')))
+         (WSAT' : wsat (r_f ⋅ (frame.(rc) ⋅ r')) σ_src' σ_tgt')
+         (* and the returned values are related w.r.t. (r ⋅ r' ⋅ r_f) *)
+         (VRET  : vrel r' (Val v_src) (Val v_tgt)),
+         ∃ idx', sim_local_body wsat vrel fns fnt
+                                (frame.(rc) ⋅ r') idx'
+                                (fill frame.(K_src) (Val v_src)) σ_src'
+                                (fill frame.(K_tgt) (Val v_tgt)) σ_tgt')
+  : sim_local_frames
+      (r_f ⋅ frame.(rc))
+      (frame.(K_src) ++ K_f_src)
+      (frame.(K_tgt) ++ K_f_tgt)
+      (frame :: frames)
+.
+
+Inductive sim_local_conf:
+  forall (idx:nat) (e_src:expr) (σ_src:state) (e_tgt:expr) (σ_tgt:state), Prop :=
+| sim_local_conf_intro
+    r_f K_src K_tgt frames
+    rc idx e_src σ_src e_tgt σ_tgt
+    Ke_src Ke_tgt
+    (FRAMES: sim_local_frames r_f K_src K_tgt frames)
+    (LOCAL: sim_local_body wsat vrel fns fnt rc idx e_src σ_src e_tgt σ_tgt)
+    (KE_SRC: Ke_src = fill K_src e_src)
+    (KE_TGT: Ke_tgt = fill K_tgt e_tgt)
+  : sim_local_conf idx Ke_src σ_src Ke_tgt σ_tgt.
+
+Lemma sim_local_conf_sim
+      (FUNS: sim_local_funs wsat vrel fns fnt)
+      (idx:nat) (e_src:expr) (σ_src:state) (e_tgt:expr) (σ_tgt:state)
+      (SIM: sim_local_conf idx e_src σ_src e_tgt σ_tgt)
+  : sim fns fnt idx (e_src, σ_src) (e_tgt, σ_tgt)
+.
+Proof.
+  revert idx e_src σ_src e_tgt σ_tgt SIM. pcofix CIH. i.
+  inv SIM. punfold LOCAL. inv LOCAL.
+  - admit.
+  - admit.
+  - admit.
+Admitted.
+
+End local.
+
+Section prog.
+Context {A: ucmraT}.
+Variable (wsat: A → state → state → Prop).
+Variable (vrel: A → expr → expr → Prop).
+Variable (fns fnt: fn_env).
+
+Lemma sim_prog_sim
+      prog_src prog_tgt
+      (FUNS: sim_local_funs wsat vrel prog_src prog_tgt)
+  : behave_prog prog_tgt <1= behave_prog prog_src.
+Proof.
+  unfold behave_prog. eapply adequacy. eapply sim_local_conf_sim; eauto.
+  econs; eauto; swap 2 4.
+  { econs 1. }
+  { ss. }
+  { ss. }
+  admit.
+Admitted.
+
+End prog.
